theory/JITFix.thy
@@ -2,6 +2,9 @@ theory JITFix
   imports JITFix_aux
 begin
 
+lemma "of_nat x - of_nat y = of_nat (x-y)"
+  value "(((of_nat 0)::u32) - (of_nat 1)::u32)"
+  value "((of_nat (0-1))::u32)"
 
 lemma jitfix_induct:
   "jitfix (a#l_jump) l_bin0 l_pc = Some prog \<Longrightarrow> 
@@ -32,11 +35,11 @@ next
     apply(split if_splits,simp_all)
     apply(cases "l_pc ! unat (snd a)",simp_all)
     subgoal for aa b
-      apply(cases "x64_decode (nat (fst (l_pc ! nat (fst a)))) l_bin0",simp_all)
+      apply(cases "x64_decode (fst (l_pc ! nat (fst a))) l_bin0",simp_all)
        subgoal for ab apply(cases ab,simp_all)
         subgoal for ac ba
           apply(cases ba,simp_all)
-           apply(cases "x64_decode (nat (fst (l_pc ! nat (fst a))) + ac) l_bin0",simp_all)
+           apply(cases "x64_decode (fst (l_pc ! nat (fst a)) + ac) l_bin0",simp_all)
           subgoal for x141 x142 ad apply(cases ad,simp_all)
             subgoal for ae bb apply(cases bb,simp_all) apply(unfold get_updated_l_bin_def x64_encode_def u8_list_of_u32_def bitfield_insert_u8_def,simp_all)
               subgoal for x131 x132               
@@ -59,48 +62,8 @@ lemma jit_fix_not_change:
   x64_decode xpc prog = Some v"
   sorry
 
-(*\<and> x64_decode 0 l \<noteq> None \<and>*)
-(*
-lemma jit_fix_change:
-  "jitfix l_jump l_bin0 l_pc = Some prog \<Longrightarrow> 
-  x64_decode xpc l_bin0 = Some v \<Longrightarrow>
-  (\<exists> num d. x64_decode xpc l_bin0 = Some(num, Pcall_i d)) \<or> (\<exists> num src dst. x64_decode xpc l_bin0 = Some(num, Pjcc cond d)) \<Longrightarrow>
-  get_updated_l_bin x l l_pc 
-  x64_decode xpc prog = x"
-*)
-
-(*
-lemma jit_fix_not_change:
-  "jitfix l_jump l_bin0 l_pc = Some prog \<Longrightarrow> 
-  x64_decode xpc l_bin0 \<noteq> None \<Longrightarrow> 
-  (\<not>(\<exists> num d. x64_decode xpc l_bin0 = Some(num, Pcall_i d))) \<and> (\<not> (\<exists> num src dst. x64_decode xpc l_bin0 = Some(num, Pjcc cond d))) \<Longrightarrow>
-  list_in_list l xpc l_bin0 \<longrightarrow> list_in_list l xpc prog"
-  sorry
-*)
-
-
-(*
-lemma jit_fix_change:
-  "jitfix l_jump l_bin0 l_pc = Some prog \<Longrightarrow> 
-  x64_decode xpc l_bin0 \<noteq> None \<Longrightarrow> 
-  (\<exists> num d. x64_decode xpc l_bin0 = Some(num, Pcall_i d)) \<or> (\<exists> num src dst. x64_decode xpc l_bin0 = Some(num, Pjcc cond d)) \<Longrightarrow>
-  list_in_list l xpc l_bin0 \<longrightarrow> list_in_list l xpc prog"
-  sorry
-
-
-lemma list_in_list_prop4: "
-  x64_sem num l_bin (Next xpc xrs xm xss) = fxst \<Longrightarrow>
-  x64_sem num lt (Next xpc xrs xm xss) = xxst \<Longrightarrow>
-  x64_bin_is_sequential (length l) l 0 \<Longrightarrow>
-  list_in_list l xpc l_bin \<Longrightarrow>
-  list_in_list l xpc lt \<Longrightarrow>
-  fxst \<noteq> Stuck \<Longrightarrow>
-  xxst = fxst"
-  sorry
-*)
-
 lemma l_pc_index_corr2:
-  "find_target_pc_in_l_pc2 l_pc (int xpc) 0 = Some pc \<Longrightarrow> nat (fst (l_pc!(nat pc))) = xpc"
+  "find_target_pc_in_l_pc2 l_pc xpc 0 = Some pc \<Longrightarrow> fst (l_pc!pc) = xpc"
   sorry
 
 
@@ -149,19 +112,19 @@ proof-
     using a0 by simp
   have c0_0:"fxst' = (case x64_decode xpc l_bin0 of 
                   Some(sz, Pcall_i imm) \<Rightarrow>
-                      let v = find_target_pc_in_l_pc2 l_pc (int xpc) 0 in
+                      let v = find_target_pc_in_l_pc2 l_pc xpc 0 in
                       (case v of None \<Rightarrow> Stuck | Some pc \<Rightarrow>
                       (case find_target_pc_in_l_pc l_jump pc of
                         None \<Rightarrow> Stuck |
                         Some npc \<Rightarrow>
-                      exec_instr (Pcall_i (of_int(fst (l_pc!(unat npc))))) sz xpc xrs xm xss)) |
+                      exec_instr (Pcall_i (of_nat(fst (l_pc!(unat npc))))) sz xpc xrs xm xss)) |
                   Some(sz, Pjcc cond d) \<Rightarrow> 
-                      let v = find_target_pc_in_l_pc2 l_pc (int xpc-3) 0 in
+                      let v = find_target_pc_in_l_pc2 l_pc (xpc-3) 0 in
                       (case v of None \<Rightarrow> Stuck | Some pc \<Rightarrow>
                       (case find_target_pc_in_l_pc l_jump pc of
                         None \<Rightarrow> Stuck |
                         Some npc \<Rightarrow>
-                          (exec_instr (Pjcc cond (of_int (fst (l_pc!(unat npc)))-(of_nat (xpc+1)))) sz xpc xrs xm xss))) |
+                          (exec_instr (Pjcc cond (of_nat(fst (l_pc!(unat npc)))-(of_nat (xpc+sz+1)))) sz xpc xrs xm xss))) |
                   Some(sz,ins) \<Rightarrow> (exec_instr ins sz xpc xrs xm xss) |
                   _ \<Rightarrow> Stuck )"
           using b0_1 a3 by(unfold fix_bpf_one_step_def Let_def,simp_all) 
@@ -169,69 +132,67 @@ proof-
   proof(cases "\<exists> num d. x64_decode xpc l_bin0 = Some(num, Pcall_i d)")
     case True
     then obtain sz d where b1:"x64_decode xpc l_bin0 = Some(sz, Pcall_i d)" by auto
-    have c0:"fxst' = (let v = find_target_pc_in_l_pc2 l_pc (int xpc) 0 in
+    have c0:"fxst' = (let v = find_target_pc_in_l_pc2 l_pc xpc 0 in
                       (case v of None \<Rightarrow> Stuck | Some pc \<Rightarrow>
                       (case find_target_pc_in_l_pc l_jump pc of
                         None \<Rightarrow> Stuck |
                         Some npc \<Rightarrow>
-                      exec_instr (Pcall_i (of_int(fst (l_pc!(unat npc))))) sz xpc xrs xm xss)))" using b1 c0_0 by simp
+                      exec_instr (Pcall_i (of_nat(fst (l_pc!(unat npc))))) sz xpc xrs xm xss)))" using b1 c0_0 by simp
     
-    hence "find_target_pc_in_l_pc2 l_pc (int xpc) 0 \<noteq> None" using a1
+    hence "find_target_pc_in_l_pc2 l_pc xpc 0 \<noteq> None" using a1
       using option.simps(4) by fastforce 
-    hence "\<exists> pc. find_target_pc_in_l_pc2 l_pc (int xpc) 0 = Some pc" by simp
-    then obtain pc where c1:"find_target_pc_in_l_pc2 l_pc (int xpc) 0 = Some pc" by auto
+    hence "\<exists> pc. find_target_pc_in_l_pc2 l_pc xpc 0 = Some pc" by simp
+    then obtain pc where c1:"find_target_pc_in_l_pc2 l_pc xpc 0 = Some pc" by auto
     hence c2_0:"find_target_pc_in_l_pc l_jump pc \<noteq> None" using c0 a1
       using option.simps(4) by fastforce 
     hence "\<exists> npc. find_target_pc_in_l_pc l_jump pc = Some npc" by force 
     then obtain npc where c2:"find_target_pc_in_l_pc l_jump pc = Some npc" by auto
-    have c3:"fxst' = exec_instr (Pcall_i (of_int(fst (l_pc!(unat npc))))) sz xpc xrs xm xss"
+    have c3:"fxst' = exec_instr (Pcall_i (of_nat(fst (l_pc!(unat npc))))) sz xpc xrs xm xss"
       using c0 c1 c2 by simp
 
-    hence d0:"(pc,npc) \<in> set l_jump" using c1 c2 search_l_jump
+    hence d0:"(int pc,npc) \<in> set l_jump" using c1 c2 search_l_jump
       by (metis a4 distinct.simps(1) init_second_layer_def is_increase_list_empty l_jump_is_distinct list.simps(8))
     have "l_bin0 \<noteq> []"
       by (metis c2_0 a2 find_target_pc_in_l_pc.simps(1) jitfix.elims option.simps(3)) 
-    hence "jitfix [(pc,npc)] l_bin0 l_pc = (let res = get_updated_l_bin (pc,npc) l_bin0 l_pc in case res of None \<Rightarrow> None | 
+    hence "jitfix [(int pc,npc)] l_bin0 l_pc = (let res = get_updated_l_bin (int pc,npc) l_bin0 l_pc in case res of None \<Rightarrow> None | 
                                                         Some l' \<Rightarrow> Some l')" by auto
-    hence d1:"jitfix [(pc,npc)] l_bin0 l_pc = get_updated_l_bin (pc,npc) l_bin0 l_pc" 
-      using a2 by(cases "get_updated_l_bin (pc,npc) l_bin0 l_pc",simp_all)
-    let "?prog" = "jitfix [(pc,npc)] l_bin0 l_pc"
-    have d2:"?prog = (let fix_begin_addr = fst (l_pc!(nat pc)); 
+    hence d1:"jitfix [(int pc,npc)] l_bin0 l_pc = get_updated_l_bin (int pc,npc) l_bin0 l_pc" 
+      using a2 by(cases "get_updated_l_bin (int pc,npc) l_bin0 l_pc",simp_all)
+    let "?prog" = "jitfix [(int pc,npc)] l_bin0 l_pc"
+    have d2:"?prog = (let fix_begin_addr = fst (l_pc!pc); 
         (target_begin_addr,num2) = l_pc!(unat npc) in 
-        (case x64_decode (nat fix_begin_addr) l_bin0 of 
-              Some(sz, Pcall_i _) \<Rightarrow> let u8_list = x64_encode (Pcall_i (of_int target_begin_addr)) in
-                                     Some (x64_bin_update (length u8_list) l_bin0 (nat fix_begin_addr) u8_list) |
-              Some(sz, Pcmpq_rr src dst) \<Rightarrow> let loc = nat fix_begin_addr+sz in 
+        (case x64_decode fix_begin_addr l_bin0 of 
+              Some(sz, Pcall_i _) \<Rightarrow> let u8_list = x64_encode (Pcall_i (of_nat target_begin_addr)) in
+                                     Some (x64_bin_update (length u8_list) l_bin0 fix_begin_addr u8_list) |
+              Some(sz, Pcmpq_rr src dst) \<Rightarrow> let loc = fix_begin_addr+sz in 
                     (case x64_decode loc l_bin0 of 
-                            Some(sz2, Pjcc cond _) \<Rightarrow> let offset = ((of_int target_begin_addr)::i32) - ((of_nat (loc+sz2)+1)::i32) in
+                            Some(sz2, Pjcc cond _) \<Rightarrow> let offset = ((of_nat target_begin_addr)::i32) - ((of_nat (loc+sz2)+1)::i32) in
                                                       let u8_list = x64_encode (Pjcc cond (ucast offset)) in                                                     
                                                       Some (x64_bin_update (length u8_list) l_bin0 loc u8_list) | 
                             _ \<Rightarrow> None ) |
               _ \<Rightarrow> None ))"
       using get_updated_l_bin_def d1 by auto
-    have d2_0:"(fst (l_pc!(nat pc))) \<ge> 0" using a3 sorry
-    have d2_1:"nat (fst (l_pc!(nat pc))) = xpc" using l_pc_index_corr2 c1 by blast     
-    have d2_2:"(fst (l_pc!(nat pc))) = int xpc" using d2_1 d2_0 by presburger     
-    have d2_3:"of_int (int xpc) = of_nat xpc" using d2_0 by simp
+    have d2_1:"fst (l_pc!pc) = xpc" using l_pc_index_corr2 c1 by blast     
+    have d2_2:"(fst (l_pc!pc)) = xpc" using d2_1 by presburger     
     let "?target_begin_addr" = "fst(l_pc!(unat npc))"
     have "?prog = (
         (case x64_decode xpc l_bin0 of 
-              Some(sz, Pcall_i _) \<Rightarrow> let u8_list = x64_encode (Pcall_i (of_int ?target_begin_addr)) in
+              Some(sz, Pcall_i _) \<Rightarrow> let u8_list = x64_encode (Pcall_i (of_nat ?target_begin_addr)) in
                                      Some (x64_bin_update (length u8_list) l_bin0 xpc u8_list) |
               Some(sz, Pcmpq_rr src dst) \<Rightarrow> let loc = xpc+sz in 
                     (case x64_decode loc l_bin0 of 
-                            Some(sz2, Pjcc cond _) \<Rightarrow> let offset = ((of_int ?target_begin_addr)::i32) - ((of_nat (loc+sz2)+1)::i32) in
+                            Some(sz2, Pjcc cond _) \<Rightarrow> let offset = ((of_nat ?target_begin_addr)::i32) - ((of_nat (loc+sz2)+1)::i32) in
                                                       let u8_list = x64_encode (Pjcc cond (ucast offset)) in                                                     
                                                       Some (x64_bin_update (length u8_list) l_bin0 loc u8_list) | 
                             _ \<Rightarrow> None ) |
               _ \<Rightarrow> None ))"
-      using d2_1 d2_2 d2_3 d2 sorry 
-    hence d3:"?prog = (let u8_list = x64_encode (Pcall_i (of_int ?target_begin_addr)) in
+      using d2_1 d2_2 d2 by (simp add: case_prod_beta) 
+    hence d3:"?prog = (let u8_list = x64_encode (Pcall_i (of_nat ?target_begin_addr)) in
                                      Some (x64_bin_update (length u8_list) l_bin0 xpc u8_list))"
       using b1 by(cases "x64_decode xpc l_bin0",simp_all)
     
-    let "?u8_list" = "(of_int ?target_begin_addr)"
-    let "?len_u8_list" = "length(x64_encode (Pcall_i (of_int ?target_begin_addr)))"
+    let "?u8_list" = "(of_nat ?target_begin_addr)"
+    let "?len_u8_list" = "length(x64_encode (Pcall_i (of_nat ?target_begin_addr)))"
     have "\<exists> someprog. ?prog = Some someprog" using a2 by (meson d3) 
     then obtain someprog where d4:"?prog = Some someprog" by auto
     hence d4_1:"Some someprog = Some (x64_bin_update (length (x64_encode (Pcall_i ?u8_list))) l_bin0 xpc (x64_encode (Pcall_i ?u8_list)))"
@@ -245,7 +206,7 @@ proof-
     have d5:"x64_decode xpc someprog = Some (?len_u8_list,Pcall_i ?u8_list)" 
       using x64_bin_update_decode_incode_consistency d4_1 by blast
     hence "?len_u8_list = sz" using b1 d5 sorry
-    (*exec_instr (Pcall_i (of_int(fst (l_pc!(unat npc))))) sz xpc xrs xm xss"*)
+    (*exec_instr (Pcall_i (of_nat(fst (l_pc!(unat npc))))) sz xpc xrs xm xss"*)
     hence d5_2:"last_fix_sem 1 someprog xst = (exec_instr (Pcall_i ?u8_list) sz xpc xrs xm xss)"
       using d5_1 d5 by simp
     hence dn:"last_fix_sem 1 someprog xst = fxst'" using d5_2 c3 by metis
@@ -268,62 +229,139 @@ proof-
     proof(cases "\<exists> num cond d. x64_decode xpc l_bin0 = Some(num, Pjcc cond d)")
       case True 
       then obtain sz cond d where b1:"x64_decode xpc l_bin0 = Some(sz, Pjcc cond d)" by auto
-      have c0:"fxst' = (let v = find_target_pc_in_l_pc2 l_pc (int xpc-3) 0 in
+      have c0:"fxst' = (let v = find_target_pc_in_l_pc2 l_pc (xpc-3) 0 in
                       (case v of None \<Rightarrow> Stuck | Some pc \<Rightarrow>
                       (case find_target_pc_in_l_pc l_jump pc of
                         None \<Rightarrow> Stuck |
                         Some npc \<Rightarrow>
-                          (exec_instr (Pjcc cond (of_int (fst (l_pc!(unat npc)))-(of_nat (xpc+1)))) sz xpc xrs xm xss))))"
+                          (exec_instr (Pjcc cond (of_nat(fst (l_pc!(unat npc)))-(of_nat (xpc+sz+1)))) sz xpc xrs xm xss))))"
         using c0_0 b1 by simp
-      have "\<exists> pc. find_target_pc_in_l_pc2 l_pc (int xpc-3) 0 = Some pc"
+      have "\<exists> pc. find_target_pc_in_l_pc2 l_pc (xpc-3) 0 = Some pc"
         using c0 a1 option.simps(4) by fastforce 
-      then obtain pc where c1:"find_target_pc_in_l_pc2 l_pc (int xpc-3) 0 = Some pc" by auto
+      then obtain pc where c1:"find_target_pc_in_l_pc2 l_pc (xpc-3) 0 = Some pc" by auto
       have "\<exists> npc. find_target_pc_in_l_pc l_jump pc = Some npc"
         using c0 c1 a1 option.exhaust_sel by fastforce
       then obtain npc where c2:"find_target_pc_in_l_pc l_jump pc = Some npc" by auto
-      have c3:"fxst' = (exec_instr (Pjcc cond (of_int (fst (l_pc!(unat npc)))-(of_nat (xpc+1)))) sz xpc xrs xm xss)"
+      have c3:"fxst' = (exec_instr (Pjcc cond (of_nat(fst (l_pc!(unat npc)))-(of_nat (xpc+sz+1)))) sz xpc xrs xm xss)"
         using c0 c2 c1 by force
 
-      have d0:"(pc,npc) \<in> set l_jump" using c2 search_l_jump
+      have d0:"(int pc,npc) \<in> set l_jump" using c2 search_l_jump
         by (metis a4 distinct.simps(1) init_second_layer_def is_increase_list_empty l_jump_is_distinct list.simps(8)) 
-      have "l_bin0 \<noteq> []" using a2
+      have d0_1:"l_bin0 \<noteq> []" using a2
         by (metis c2 find_target_pc_in_l_pc.simps(1) jitfix.simps(2) list.exhaust option.distinct(1)) 
-       hence "jitfix [(pc,npc)] l_bin0 l_pc = (let res = get_updated_l_bin (pc,npc) l_bin0 l_pc in case res of None \<Rightarrow> None | 
+       hence "jitfix [(int pc,npc)] l_bin0 l_pc = (let res = get_updated_l_bin (int pc,npc) l_bin0 l_pc in case res of None \<Rightarrow> None | 
                                                         Some l' \<Rightarrow> Some l')" by auto
-    hence d1:"jitfix [(pc,npc)] l_bin0 l_pc = get_updated_l_bin (pc,npc) l_bin0 l_pc" 
-      using a2 by(cases "get_updated_l_bin (pc,npc) l_bin0 l_pc",simp_all)
-    let "?prog" = "jitfix [(pc,npc)] l_bin0 l_pc"
-    have d2:"?prog = (let fix_begin_addr = fst (l_pc!(nat pc)); 
+    hence d1:"jitfix [(int pc,npc)] l_bin0 l_pc = get_updated_l_bin (int pc,npc) l_bin0 l_pc" 
+      using a2 by(cases "get_updated_l_bin (int pc,npc) l_bin0 l_pc",simp_all)
+    let "?prog" = "jitfix [(int pc,npc)] l_bin0 l_pc"
+    have d2:"?prog = (let fix_begin_addr = fst (l_pc!pc); 
         (target_begin_addr,num2) = l_pc!(unat npc) in 
-        (case x64_decode (nat fix_begin_addr) l_bin0 of 
-              Some(sz, Pcall_i _) \<Rightarrow> let u8_list = x64_encode (Pcall_i (of_int target_begin_addr)) in
-                                     Some (x64_bin_update (length u8_list) l_bin0 (nat fix_begin_addr) u8_list) |
-              Some(sz, Pcmpq_rr src dst) \<Rightarrow> let loc = nat fix_begin_addr+sz in 
+        (case x64_decode fix_begin_addr l_bin0 of 
+              Some(sz, Pcall_i _) \<Rightarrow> let u8_list = x64_encode (Pcall_i (of_nat target_begin_addr)) in
+                                     Some (x64_bin_update (length u8_list) l_bin0 fix_begin_addr u8_list) |
+              Some(sz, Pcmpq_rr src dst) \<Rightarrow> let loc = fix_begin_addr+sz in 
                     (case x64_decode loc l_bin0 of 
-                            Some(sz2, Pjcc cond _) \<Rightarrow> let offset = ((of_int target_begin_addr)::i32) - ((of_nat (loc+sz2)+1)::i32) in
+                            Some(sz2, Pjcc cond _) \<Rightarrow> let offset = ((of_nat target_begin_addr)::i32) - ((of_nat (loc+sz2)+1)::i32) in
                                                       let u8_list = x64_encode (Pjcc cond (ucast offset)) in                                                     
                                                       Some (x64_bin_update (length u8_list) l_bin0 loc u8_list) | 
                             _ \<Rightarrow> None ) |
               _ \<Rightarrow> None ))"
       using get_updated_l_bin_def d1 by auto
-    have d2_0:"(fst (l_pc!(nat pc))) \<ge> 0" using a3 sorry
-    have d2_1:"nat (fst (l_pc!(nat pc))) = xpc" using l_pc_index_corr2 c1 sorry
-    have d2_2:"(fst (l_pc!(nat pc))) = int xpc" using d2_1 d2_0 by presburger     
-    have d2_3:"of_int (int xpc) = of_nat xpc" using d2_0 by simp
-    let "?target_begin_addr" = "fst(l_pc!(unat npc))"
-    have "?prog = (
-        (case x64_decode xpc l_bin0 of 
-              Some(sz, Pcall_i _) \<Rightarrow> let u8_list = x64_encode (Pcall_i (of_int ?target_begin_addr)) in
-                                     Some (x64_bin_update (length u8_list) l_bin0 xpc u8_list) |
-              Some(sz, Pcmpq_rr src dst) \<Rightarrow> let loc = xpc+sz in 
+
+    have d3_1:"?prog \<noteq> None" sorry
+    have d3_0_0:"fst (l_pc!pc) = xpc-3"
+      using c1 l_pc_index_corr2 by blast 
+    hence d3_0_1:"fst (l_pc!pc)+3 = (xpc-3)+3" using d3_0_0 by presburger 
+    moreover have d3_0_2:"xpc-3\<ge>0" by blast
+    hence d3_0:"fst (l_pc!pc) +3 = xpc" using d3_0_1 d3_0_2 sorry
+    have d3_2:"x64_decode (fst (l_pc!pc)) l_bin0 \<noteq> None" using d2 a2 d0_1 d3_1 by(cases "x64_decode (fst (l_pc!pc)) l_bin0",simp_all)
+    hence "(\<exists> sz d. x64_decode (fst (l_pc!pc)) l_bin0 = Some(sz, Pcall_i d)) \<or> (\<exists> sz src dst. x64_decode (fst (l_pc!pc)) l_bin0 = Some(sz, Pcmpq_rr src dst))"
+      using d2 a2 d0_1 d3_1 apply(cases "x64_decode (fst (l_pc!pc)) l_bin0",simp_all)
+      subgoal for a apply(cases "get_updated_l_bin (int pc, npc) l_bin0 l_pc",simp_all)
+        subgoal for aa apply(cases "l_pc ! unat npc",simp_all)
+          subgoal for ab b apply(cases a,simp_all)
+            subgoal for ac ba apply(cases ba,simp_all)
+              done
+            done
+          done
+        done
+      done
+    then obtain sz1 d sz2 src dst where d4:"x64_decode (fst (l_pc!pc)) l_bin0 = Some(sz1, Pcall_i d) \<or> x64_decode (fst (l_pc!pc)) l_bin0 = Some(sz2, Pcmpq_rr src dst)" by auto
+    thus ?thesis 
+    proof(cases "x64_decode (fst (l_pc!pc)) l_bin0 = Some(sz2, Pcmpq_rr src dst)")
+      case True
+      have d5:"?prog = (
+        let (target_begin_addr,num2) = l_pc!(unat npc) in 
+        (let loc = (fst (l_pc!pc))+sz2 in 
                     (case x64_decode loc l_bin0 of 
-                            Some(sz2, Pjcc cond _) \<Rightarrow> let offset = ((of_int ?target_begin_addr)::i32) - ((of_nat (loc+sz2)+1)::i32) in
+                            Some(sz2, Pjcc cond _) \<Rightarrow> let offset = ((of_nat target_begin_addr)::i32) - ((of_nat (loc+sz2)+1)::i32) in
                                                       let u8_list = x64_encode (Pjcc cond (ucast offset)) in                                                     
-                                                      Some (x64_bin_update (length u8_list) l_bin0 loc u8_list) | 
-                            _ \<Rightarrow> None ) |
-              _ \<Rightarrow> None ))"
-      using d2_1 d2_2 d2_3 d2 sorry 
-      thus ?thesis sorry
+                                                      Some (x64_bin_update (length u8_list) l_bin0 loc u8_list))))"
+        using d2 d3_1 True d0_1 d3_2 d4 apply(unfold Let_def,simp_all)
+        apply(cases "get_updated_l_bin (int pc, npc) l_bin0 l_pc",simp_all)
+        subgoal for a  apply(cases "l_pc ! unat npc",simp_all)
+          subgoal for aa b apply(cases "x64_decode (fst (l_pc!pc)) l_bin0",simp_all)
+            subgoal for ab apply(unfold Let_def,simp_all)
+              apply(cases "x64_decode (fst (l_pc ! pc) + sz2) l_bin0",simp_all)
+              subgoal for ac apply(cases ac,simp_all)
+                subgoal for ad ba apply(cases ba,simp_all)
+                  done
+                done
+              done
+            done
+          done
+        done
+      let "?target_begin_addr" = "fst(l_pc!(unat npc))"
+
+      let "?loc" = "(fst (l_pc!pc))+sz2"
+      have "sz2 = 3" sorry
+      hence d5_1:"?loc = xpc" using d3_0 by force  
+      let "?offset" = "((of_nat ?target_begin_addr)::i32) - ((of_nat (xpc+sz)+1)::i32)"
+      let "?u8_list" = "Pjcc cond (ucast ?offset)"
+      let "?len_u8_list" = "length(x64_encode (Pjcc cond (ucast ?offset)))"
+
+      have d6:"?prog = Some (x64_bin_update (length (x64_encode ?u8_list)) l_bin0 ?loc (x64_encode ?u8_list))"
+        using d5 d0_1 d3_1 b1 d5_1 apply(unfold Let_def,simp_all)
+        apply(cases "get_updated_l_bin (int pc, npc) l_bin0 l_pc",simp_all)
+        subgoal for a apply(unfold Let_def,simp_all)
+          apply(cases "l_pc ! unat npc",simp_all)
+          done
+        done
+        
+      have "\<exists> someprog. ?prog = Some someprog" using a2 d3_1 by auto
+      then obtain someprog where d4:"?prog = Some someprog" by auto
+      have d7:"x64_decode xpc someprog = Some (?len_u8_list,?u8_list)"
+        using d4 d5_1 d6 x64_bin_update_decode_incode_consistency by presburger 
+     
+      have d8_1:"last_fix_sem 1 someprog xst = (x64_sem 1 someprog xst)" using last_fix_sem_def by blast
+      hence d8_2:"last_fix_sem 1 someprog xst = (case x64_decode xpc someprog of
+        None \<Rightarrow> Stuck |
+        Some (sz, ins) \<Rightarrow>
+         (exec_instr ins sz xpc xrs xm xss))" using a3
+        by (simp add: option.case_eq_if)  
+
+      have "?len_u8_list = sz" sorry
+                                (* "fxst' = (exec_instr (Pjcc cond (of_nat(fst (l_pc!(unat npc)))-(of_nat (xpc+sz+1)))) sz xpc xrs xm xss)"*)
+      hence dn:"last_fix_sem 1 someprog xst = ((exec_instr (Pjcc cond (ucast((of_nat ?target_begin_addr)::i32) - ((of_nat (xpc+sz)+1)::i32))) sz xpc xrs xm xss))" 
+        using d7 d8_2 last_fix_sem_def by force 
+
+      
+      have e0:"last_fix_sem 1 prog xst = (case x64_decode xpc prog of
+      None \<Rightarrow> Stuck |
+      Some (sz, ins) \<Rightarrow>
+       (exec_instr ins sz xpc xrs xm xss))" using a3 last_fix_sem_def by (simp add: option.case_eq_if)  
+
+      have e1:"x64_decode xpc someprog = x64_decode xpc prog" using d7 a2 d0 d4 d5_1 d6 x64_bin_update_is_disjoint by presburger 
+
+      have e2:"last_fix_sem 1 prog xst = (exec_instr (Pjcc cond (ucast((of_nat ?target_begin_addr)::i32) - ((of_nat (xpc+sz)+1)::i32))) sz xpc xrs xm xss)"
+        using e0 e1 dn d8_2 by argo  
+
+      then show ?thesis using match_state2_def c3 dn d4
+        by (metis (mono_tags, lifting) a1 a7 of_nat_1 of_nat_add outcome.distinct(1) ucast_id) 
+    next
+      case False
+      then show ?thesis sorry
+    qed
       (*have c0_0:"\<exists> num src dst. x64_decode xpc l_bin0 = Some(num, Pjcc cond d)" using True by simp
       then obtain num src dst where c0_1:"x64_decode xpc l_bin0 = Some(num, Pcmpq_rr src dst)" by auto
       have c0:"snd fxst' = snd (let num = snd (l_pc!(unat pc)) in case x64_sem num l_bin0 (Next xpc xrs xm xss) of
@@ -378,10 +416,10 @@ proof-
                   by(cases "get_updated_l_bin (uint pc,npc) l_bin0 l_pc",simp_all)
                 hence d1:"jitfix [(uint pc,npc)] l_bin0 l_pc = (let fix_begin_addr = fst (l_pc!(nat(uint pc))); 
         (target_begin_addr,num2) = l_pc!(unat npc) in 
-        (case x64_decode (nat fix_begin_addr) l_bin0 of 
+        (case x64_decode fix_begin_addr l_bin0 of 
               Some(sz, Pcall_i _) \<Rightarrow> let offset = ((of_int target_begin_addr)::i32) - ((of_int fix_begin_addr+of_nat sz+1)::i32) in 
                                      let u8_list = x64_encode (Pcall_i (ucast offset)) in
-                                     Some (x64_bin_update (length u8_list) l_bin0 (nat fix_begin_addr) u8_list) |
+                                     Some (x64_bin_update (length u8_list) l_bin0 fix_begin_addr u8_list) |
               Some(sz, Pcmpq_rr src dst) \<Rightarrow> let loc = nat fix_begin_addr+sz in 
                     (case x64_decode loc l_bin0 of 
                             Some(sz2, Pjcc cond _) \<Rightarrow> let offset = ((of_int target_begin_addr)::i32) - ((of_nat (loc+sz2)+1)::i32) in
@@ -397,7 +435,7 @@ proof-
                 then obtain sz src dst where d3_1:"x64_decode (nat ?fix_begin_addr) l_bin0 = Some(sz, Pcmpq_rr src dst)" by auto
                 hence d3:"jitfix [(uint pc,npc)] l_bin0 l_pc =  (let loc = nat ?fix_begin_addr+sz in 
                     (case x64_decode loc l_bin0 of 
-                            Some(sz2, Pjcc cond _) \<Rightarrow> let offset = ((of_int ?target_begin_addr)::i32) - ((of_nat (loc+sz2)+1)::i32) in
+                            Some(sz2, Pjcc cond _) \<Rightarrow> let offset = ((of_nat ?target_begin_addr)::i32) - ((of_nat (loc+sz2)+1)::i32) in
                                                       let u8_list = x64_encode (Pjcc cond (ucast offset)) in                                                     
                                                       Some (x64_bin_update (length u8_list) l_bin0 loc u8_list) | 
                             _ \<Rightarrow> None ))" using d1 d2 d1_1
@@ -430,7 +468,7 @@ proof-
                 then obtain prog' where "Some prog' = jitfix [(uint pc,npc)] l_bin0 l_pc" by auto
                 hence "prog' = (let loc = nat ?fix_begin_addr+sz in 
                     (case x64_decode loc l_bin0 of 
-                            Some(sz2, Pjcc cond _) \<Rightarrow> let offset = ((of_int ?target_begin_addr)::i32) - ((of_nat (loc+sz2)+1)::i32) in
+                            Some(sz2, Pjcc cond _) \<Rightarrow> let offset = ((of_nat ?target_begin_addr)::i32) - ((of_nat (loc+sz2)+1)::i32) in
                                                       let u8_list = x64_encode (Pjcc cond (ucast offset)) in                                                     
                                                       (x64_bin_update (length u8_list) l_bin0 loc u8_list)))"
                   using d3 apply(cases "x64_decode (nat ?fix_begin_addr+sz) l_bin0",simp_all)
@@ -513,142 +551,7 @@ proof-
       qed
     qed
 
-(*
-(*(l_bin0,l_pc,l_jump) *)
-lemma n_steps_equiv_layer2:
-  "flat_bpf_sem n (l_bin0,l_pc,l_jump) (pc,xst) = fxst' \<Longrightarrow>
-  xst = Next xpc xrs xm xss \<Longrightarrow>
-  snd fxst' = Next xpc'' xrs'' xm'' xss'' \<Longrightarrow>
-  jitfix l_jump l_bin0 l_pc = Some prog \<Longrightarrow>
-  jitflat_bpf lt init_second_layer = (l_bin0,l_pc,l_jump) \<Longrightarrow>
-  well_formed_prog lt \<Longrightarrow>
-  \<exists> num fst'. last_fix_sem num prog xst = fst' \<and> match_state2 fst' (snd fxst')"
-proof(induct n arbitrary:l_bin0 l_pc l_jump pc xst fxst' xpc xrs xm xss xpc'' xrs'' xm'' xss'' prog lt)
-  case 0 
-  assume assm0:"flat_bpf_sem 0 (l_bin0,l_pc,l_jump) (pc,xst) = fxst'" and
-    assm1:"xst = Next xpc xrs xm xss" and
-    assm2:"snd fxst' = Next xpc'' xrs'' xm'' xss''" and
-    assm3:"jitfix l_jump l_bin0 l_pc = Some prog" and
-    assm4:"jitflat_bpf lt init_second_layer = (l_bin0,l_pc,l_jump)" and
-    assm5:"well_formed_prog lt" 
-  have a0:"last_fix_sem 0 prog xst = xst"  by (simp add: last_fix_sem_def) 
-  have a1:"snd (flat_bpf_sem 0 (l_bin0,l_pc,l_jump) (pc,xst)) = xst" by simp
 
-  have "\<exists> num fst'. num = 0 \<and> last_fix_sem num prog xst = fst'" using a0 by blast
-
-  hence "\<exists> num fst'. num = 0 \<and> last_fix_sem num prog xst = fst' \<and> match_state2 fst' (snd fxst')"
-  using a0 a1 apply(unfold match_state2_def last_fix_sem_def,simp_all) 
-    using assm1 assm0 apply(cases fxst') 
-    subgoal for a b apply(cases fxst')
-      subgoal for aa ba apply(cases xst)
-        subgoal for x11 x12 x13 x14 apply(cases xst,simp_all)
-          subgoal for x11a by(cases b,simp_all)
-          done
-        apply(cases xst,simp_all)
-          done
-        done
-      done
-           
-  then show ?case by blast
-    (*by (smt (verit, ccfv_threshold) flat_bpf_sem.simps(1) last_fix_sem_def match_state2_def outcome.simps(4) snd_conv x64_sem.simps(1))*) 
-next
-  case (Suc n)
-  assume assm0:"flat_bpf_sem (Suc n) (l_bin0,l_pc,l_jump) (pc,xst) = fxst'" and
-    assm1:"xst = Next xpc xrs xm xss" and
-    assm2:"snd fxst' = Next xpc'' xrs'' xm'' xss''" and
-    assm3:"jitfix l_jump l_bin0 l_pc = Some prog"
-  have "\<exists> next_f. flat_bpf_sem 1 (l_bin0,l_pc,l_jump) (pc,xst) = next_f" by blast
-  then obtain next_f where b0:"flat_bpf_sem 1 (l_bin0,l_pc,l_jump) (pc,xst) = next_f" by auto
-  have "unat pc < length lt \<and> unat pc \<ge> 0" 
-  proof(rule ccontr)
-    assume assm:"\<not> (unat pc < length lt \<and> unat pc \<ge> 0)"
-    have "snd next_f = snd (let pair = flat_bpf_one_step (l_bin0,l_pc,l_jump) (pc, xst) in
-    flat_bpf_sem 0 (l_bin0,l_pc,l_jump) pair)" 
-      using b0 by fastforce
-    hence "snd next_f = snd (flat_bpf_one_step (l_bin0,l_pc,l_jump) (pc, xst))"
-      by (metis flat_bpf_sem.simps(1) prod.collapse) 
-    hence "snd next_f = Stuck" 
-      using flat_bpf_one_step_def assm assm2 apply(cases xst,simp_all)
-      subgoal for x11 x12 x13 x14 apply(cases "(l_bin0,l_pc,l_jump)",simp_all)
-        subgoal for a 
-          by (smt (z3) Suc.prems(5) add.right_neutral init_second_layer_def l_pc_length_prop list.size(3) nat_le_linear nat_less_le)
-        done
-      done
-      thus "False" using assm2
-        by (metis assm0 b0 err_is_still_err3 flat_bpf_sem_induct_aux2 outcome.distinct(1) prod.collapse) 
-  qed
-
-  hence "\<exists> num next_s. last_fix_sem num prog xst = next_s \<and> match_state2 next_s (snd next_f)"
-    using one_steps_equiv_layer2 b0 assm0 assm2 assm3 flat_bpf_sem_induct_aux2 intermediate_step_is_ok3
-    by (metis (no_types, lifting) One_nat_def Suc.prems(2) Suc.prems(5) Suc.prems(6) less_eq_nat.simps(1) old.prod.exhaust snd_conv)  
-  then obtain num next_s where b1:"last_fix_sem num prog xst = next_s \<and> match_state2 next_s (snd next_f)" by auto
-  have "\<exists> xpc' xrs' xm' xss'. snd next_f = Next xpc' xrs' xm' xss'"
-    by (metis Suc.prems(3) assm0 b0 flat_bpf_sem_induct_aux2 intermediate_step_is_ok3 less_eq_nat.simps(1) outcome.distinct(1) prod.collapse)
-  then obtain xpc' xrs' xm' xss' where b2:"snd next_f = Next xpc' xrs' xm' xss'" by auto
-  have b3:"flat_bpf_sem n (l_bin0,l_pc,l_jump) next_f = fxst'" using flat_bpf_sem_induct_aux2 b0 assm0 by blast 
-  have "flat_bpf_sem n (l_bin0, l_pc, l_jump) (pc, xst) = fxst' \<Longrightarrow>
-      xst = Next xpc xrs xm xss \<Longrightarrow> 
-      snd fxst' = Next xpc'' xrs'' xm'' xss'' \<Longrightarrow> 
-      jitfix l_jump l_bin0 l_pc = Some prog \<Longrightarrow> 
-      \<exists>(num::nat) fst'::outcome. last_fix_sem num prog xst = fst' \<and> match_state2 fst' (snd fxst')" using Suc by simp
-  hence "\<exists>(num::nat) fst'::outcome. last_fix_sem num prog (snd next_f) = fst' \<and> match_state2 fst' (snd fxst')" 
-    using b2 b1 match_state2_def assm3 b0 assm2 b3
-    by (metis Suc.hyps Suc.prems(5) Suc.prems(6) prod.collapse) 
-    
-  then show ?case
-    by (metis Suc.prems(2) b1 last_fix_sem_def match_state2_def x64_sem_add) 
-qed
-
-
-lemma n_steps_equiv:
-  assumes assm0:"perir_sem n lt (pc,xxst) = xxst'" and
-  assm1:"xxst = Next xpc xrs xm xss" and
-  assm2:"snd xxst' = Next xpc' xrs' xm' xss'" and
-  assm3:"JITFlattern_def.match_state (pc,xxst) (pc,fxst)" and
-  assm4:"lt \<noteq> []" and
-  assm5:"well_formed_prog lt"and
-
-  assm6:"jitflat_bpf lt init_second_layer = (l_bin0,l_pc,l_jump)" and
-  assm7:"flat_bpf_sem n (l_bin0,l_pc,l_jump) (pc,fxst) = fxst'" and
-  assm8:"snd fxst' = Next xpc'' xrs'' xm'' xss''" and
-
-  assm9:"jitfix l_jump l_bin0 l_pc = Some prog" and
-  (*assm10:"last_fix_sem n prog xst = fst'" and*)
-  assm11:"jitper insns = Some lt"
-  shows "\<exists> num fst'. last_fix_sem num prog fxst = fst' \<and> match_state1 fst' (snd xxst')"
-proof-
-  have b0:"JITFlattern_def.match_state xxst' fxst'" 
-    using n_steps_equiv_layer1 assm3 assm0 assm1 assm2 assm4 assm5 assm11 assm6 assm7 assm8 by auto 
-  have "\<exists> xpc1 xrs xm xss. fxst = Next xpc1 xrs xm xss" 
-    using JITFlattern_def.match_state_def assm1 assm3 
-    apply(cases xxst,simp_all) 
-    apply(cases fxst,simp_all)
-    done
-  then obtain xpc1 xrs xm xss where b1:"fxst = Next xpc1 xrs xm xss" by auto
-  have b2:"\<exists> num fst'. last_fix_sem num prog fxst = fst' \<and> match_state2 fst' (snd fxst')" 
-    using n_steps_equiv_layer2 assm7 assm9 b1 assm8 assm6 assm5 by blast
-  then obtain num fst' where b3:"last_fix_sem num prog fxst = fst' \<and> match_state2 fst' (snd fxst')" by auto
-  hence b4:"match_state1 fst' (snd xxst')"
-    apply(unfold JITFlattern_def.match_state_def match_state2_def,simp_all)
-    using assm2 assm8 b0 b3
-    apply(cases fst',simp_all)
-    apply(cases "snd fxst'",simp_all)
-    apply(cases "snd xxst'",simp_all) 
-    subgoal for x11 x11a 
-      apply(cases "snd fxst'",simp_all)
-      subgoal for x11b
-        apply(unfold JITFlattern_def.match_state_def match_state2_def match_state1_def,simp_all)
-        apply(cases xxst',simp_all)
-        subgoal for a b 
-          apply(cases fxst',simp_all)
-          done
-        done
-      done
-    done
-  have "\<exists> num fst'. last_fix_sem num prog fxst = fst' \<and> match_state1 fst' (snd xxst')" using b2 b4 b3 by blast
-  thus ?thesis using b2 by auto
-qed
-*)
 
 lemma n_steps_equiv_layer3:
   "fix_bpf_sem n (l_bin0,l_pc,l_jump) xst = fxst' \<Longrightarrow>
@@ -743,284 +646,6 @@ proof-
   thus ?thesis using b2 by auto
 qed
 
-(*num = snd (l_pc!(unat pc))*)
-(*
-lemma one_steps_equiv_layer2:
-  "flat_bpf_sem 1 (l_bin0,l_pc,l_jump) (pc,xst) = fxst' \<Longrightarrow>
-  xst = Next xpc xrs xm xss \<Longrightarrow>
-  snd fxst' = Next xpc'' xrs'' xm'' xss'' \<Longrightarrow>
-  jitfix l_jump l_bin0 l_pc = Some prog \<Longrightarrow>  
-  jitflat_bpf lt init_second_layer = (l_bin0,l_pc,l_jump) \<Longrightarrow>
-  well_formed_prog lt \<Longrightarrow>
-  unat pc < length lt \<and> unat pc \<ge> 0 \<Longrightarrow>
-  \<exists> num fst'. last_fix_sem num prog xst = fst' \<and> match_state2 fst' (snd fxst')"
-proof-
-  assume a0:"flat_bpf_sem 1 (l_bin0,l_pc,l_jump) (pc,xst) = fxst'" and
-  a1:"snd fxst' = Next xpc'' xrs'' xm'' xss''" and
-  a2:"jitfix l_jump l_bin0 l_pc = Some prog" and
-  a3:"xst = Next xpc xrs xm xss" and
-  a4:"jitflat_bpf lt init_second_layer = (l_bin0,l_pc,l_jump)" and
-  a5:"well_formed_prog lt" and
-  a6:"unat pc < length lt \<and> unat pc \<ge> 0"
-
-  have "snd fxst' =  snd (let pair = flat_bpf_one_step (l_bin0,l_pc,l_jump) (pc, xst) in flat_bpf_sem 0 (l_bin0,l_pc,l_jump) pair)"
-            using a0 by simp
-  hence b0_1:"snd fxst' =  snd (flat_bpf_one_step (l_bin0,l_pc,l_jump) (pc, xst))" by (metis flat_bpf_sem.simps(1) prod.collapse)
-  have b0_3:"unat pc < length l_pc" using l_pc_length_prop a4 init_second_layer_def
-    by (metis Nat.add_0_right a6 list.size(3)) 
-  have b0_2:"nat (fst (l_pc!(unat pc))) = xpc" using a1 b0_1 b0_3 a3 flat_bpf_one_step_def sorry
-
-  thus ?thesis 
-  proof(cases "\<exists> num d. x64_decode xpc l_bin0 = Some(num, Pcall_i d)")
-    case True
-    then show ?thesis sorry
-  next
-    case False
-    have b0:"\<not>(\<exists> num d. x64_decode xpc l_bin0 = Some(num, Pcall_i d))" using False by simp
-    then show ?thesis
-    proof(cases "\<exists> num src dst. x64_decode xpc l_bin0 = Some(num, Pcmpq_rr src dst)")
-      case True
-      have c0_0:"\<exists> num src dst. x64_decode xpc l_bin0 = Some(num, Pcmpq_rr src dst)" using True by simp
-      then obtain num src dst where c0_1:"x64_decode xpc l_bin0 = Some(num, Pcmpq_rr src dst)" by auto
-      have c0:"snd fxst' = snd (let num = snd (l_pc!(unat pc)) in case x64_sem num l_bin0 (Next xpc xrs xm xss) of
-          Stuck \<Rightarrow> (pc, Stuck) | \<comment>\<open> if one step error, stop, it should be impossible \<close>
-          Next xpc1 rs1 m1 ss1 \<Rightarrow> (
-            if rs1 (CR ZF) = 1 then \<comment>\<open> must JUMP \<close>
-              (case find_target_pc_in_l_pc l_jump (uint pc) of
-              None \<Rightarrow> (pc, Stuck) |
-              Some npc \<Rightarrow>
-                (npc, (Next (nat (fst (l_pc!(unat npc)))) rs1 m1 ss1))) \<comment>\<open> go to the target address in the jited x64 binary \<close>
-            else \<comment>\<open> donot JUMP \<close>
-              (pc+1, (Next xpc1 rs1 m1 ss1))
-          ))" using True a0 b0_1 a3 a6 b0_3 a1
-        apply(unfold flat_bpf_one_step_def Let_def,simp_all) 
-        apply(cases "x64_decode xpc l_bin0",simp_all)
-        subgoal for a apply(split if_splits,simp_all)
-          done
-        done
-      let "?num" = "(snd (l_pc!(unat pc)))"
-      have "\<exists> fxst1. fxst1 = x64_sem ?num l_bin0 (Next xpc xrs xm xss)" by fastforce
-      then obtain fxst1 where c1:"fxst1 = x64_sem ?num l_bin0 (Next xpc xrs xm xss)" by auto
-      have "fxst1 \<noteq> Stuck" using c0 a1 c1 by(cases "x64_sem ?num l_bin0 (Next xpc xrs xm xss)",simp_all)
-      hence "\<exists> xpc1 xrs1 xm1 xss1. Next xpc1 xrs1 xm1 xss1 = fxst1"
-        by (metis outcome.exhaust) 
-      then obtain xpc1 xrs1 xm1 xss1 where c2:"Next xpc1 xrs1 xm1 xss1 = fxst1" by auto
-      have c3_0:"snd fxst' = snd (if xrs1 (CR ZF) = 1 then \<comment>\<open> must JUMP \<close>
-              (case find_target_pc_in_l_pc l_jump (uint pc) of
-              None \<Rightarrow> (pc, Stuck) |
-              Some npc \<Rightarrow>
-                (npc, (Next (nat (fst (l_pc!(unat npc)))) xrs1 xm1 xss1))) \<comment>\<open> go to the target address in the jited x64 binary \<close>
-            else \<comment>\<open> donot JUMP \<close>
-              (pc+1, (Next xpc1 xrs1 xm1 xss1))
-          )" using c2 c1 c0
-        by (metis (no_types, lifting) outcome.simps(4)) 
-      thus ?thesis
-      proof(cases "xrs1 (CR ZF) = 1")
-        case True
-        have b1:"xrs1 (CR ZF) = 1" using True by simp
-        then show ?thesis
-            proof(cases "find_target_pc_in_l_pc l_jump (uint pc) \<noteq> None")
-              case True
-                have "\<exists> npc. find_target_pc_in_l_pc l_jump (uint pc) = Some npc" using True by simp
-                then obtain npc where c3_1:"find_target_pc_in_l_pc l_jump (uint pc) = Some npc" by auto                                 
-                have c3:"snd fxst' = (Next (nat (fst (l_pc!(unat npc)))) xrs1 xm1 xss1)" 
-                  using True c3_0 c3_1 b1 by simp
-                have "distinct (map fst l_jump)" using init_second_layer_def a4 is_increase_list_empty
-                  by (metis distinct.simps(1) l_jump_is_distinct list.simps(8)) 
-                hence d0:"(uint pc,npc) \<in> set l_jump" using c3_1 search_l_jump by auto
-                have d1_1:"l_bin0 \<noteq> []" using a2
-                  by (metis True find_target_pc_in_l_pc.simps(1) jitfix.elims option.distinct(1)) 
-                hence "jitfix [(uint pc,npc)] l_bin0 l_pc = get_updated_l_bin (uint pc,npc) l_bin0 l_pc" 
-                  by(cases "get_updated_l_bin (uint pc,npc) l_bin0 l_pc",simp_all)
-                hence d1:"jitfix [(uint pc,npc)] l_bin0 l_pc = (let fix_begin_addr = fst (l_pc!(nat(uint pc))); 
-        (target_begin_addr,num2) = l_pc!(unat npc) in 
-        (case x64_decode (nat fix_begin_addr) l_bin0 of 
-              Some(sz, Pcall_i _) \<Rightarrow> let offset = ((of_int target_begin_addr)::i32) - ((of_int fix_begin_addr+of_nat sz+1)::i32) in 
-                                     let u8_list = x64_encode (Pcall_i (ucast offset)) in
-                                     Some (x64_bin_update (length u8_list) l_bin0 (nat fix_begin_addr) u8_list) |
-              Some(sz, Pcmpq_rr src dst) \<Rightarrow> let loc = nat fix_begin_addr+sz in 
-                    (case x64_decode loc l_bin0 of 
-                            Some(sz2, Pjcc cond _) \<Rightarrow> let offset = ((of_int target_begin_addr)::i32) - ((of_nat (loc+sz2)+1)::i32) in
-                                                      let u8_list = x64_encode (Pjcc cond (ucast offset)) in                                                     
-                                                      Some (x64_bin_update (length u8_list) l_bin0 loc u8_list) | 
-                            _ \<Rightarrow> None ) |
-              _ \<Rightarrow> None ))" using get_updated_l_bin_def by simp
-
-                let "?fix_begin_addr" = "fst (l_pc!(nat(uint pc)))"
-                let "?target_begin_addr" = "fst (l_pc!(unat npc))"
-                have d2:"nat ?fix_begin_addr = xpc" using b0_2 by auto
-                hence "\<exists> sz src dst. x64_decode (nat ?fix_begin_addr) l_bin0 = Some(sz, Pcmpq_rr src dst)" using c0_0 by force 
-                then obtain sz src dst where d3_1:"x64_decode (nat ?fix_begin_addr) l_bin0 = Some(sz, Pcmpq_rr src dst)" by auto
-                hence d3:"jitfix [(uint pc,npc)] l_bin0 l_pc =  (let loc = nat ?fix_begin_addr+sz in 
-                    (case x64_decode loc l_bin0 of 
-                            Some(sz2, Pjcc cond _) \<Rightarrow> let offset = ((of_int ?target_begin_addr)::i32) - ((of_nat (loc+sz2)+1)::i32) in
-                                                      let u8_list = x64_encode (Pjcc cond (ucast offset)) in                                                     
-                                                      Some (x64_bin_update (length u8_list) l_bin0 loc u8_list) | 
-                            _ \<Rightarrow> None ))" using d1 d2 d1_1
-                  apply(cases "x64_decode (nat ?fix_begin_addr) l_bin0",simp_all)
-                  subgoal for a apply(cases "l_pc ! unat npc",simp_all)
-                    subgoal for aa b
-                    proof -
-                      assume "nat (fst (l_pc ! unat pc)) = xpc"
-                      assume "(case get_updated_l_bin (uint pc, npc) l_bin0 l_pc of None \<Rightarrow> None | Some x \<Rightarrow> Some x) = 
-                          (let loc = xpc + sz in case x64_decode loc l_bin0 of None \<Rightarrow> None | Some (sz2, Pjcc cond x) \<Rightarrow> 
-                           let offset = word_of_int aa - (word_of_nat (loc + sz2) + (1::32 signed word)); 
-                               u8_list = x64_encode (Pjcc cond (ucast offset)) in Some (x64_bin_update (length u8_list) l_bin0 loc u8_list) | Some (sz2, _) \<Rightarrow> None)"
-                      assume a1: "l_pc ! unat npc = (aa, b)"
-                      have "\<forall>i n. fst (i::int, n::nat) = i"
-                        by simp
-                      then show ?thesis
-                        using a1 by presburger
-                    qed 
-                    done
-                  done
-                have "jitfix [(uint pc,npc)] l_bin0 l_pc \<noteq> None"
-                proof(rule ccontr)
-                  assume assm:"\<not> (jitfix [(uint pc,npc)] l_bin0 l_pc\<noteq> None)"
-                  have "jitfix [(uint pc,npc)] l_bin0 l_pc = None" using assm by simp
-                  hence "jitfix l_jump l_bin0 l_pc = None " using d0 sorry
-                  thus "False" using a2 by simp
-                qed
-                hence "\<exists> prog'. Some prog' = jitfix [(uint pc,npc)] l_bin0 l_pc"
-                  by force
-                then obtain prog' where "Some prog' = jitfix [(uint pc,npc)] l_bin0 l_pc" by auto
-                hence "prog' = (let loc = nat ?fix_begin_addr+sz in 
-                    (case x64_decode loc l_bin0 of 
-                            Some(sz2, Pjcc cond _) \<Rightarrow> let offset = ((of_int ?target_begin_addr)::i32) - ((of_nat (loc+sz2)+1)::i32) in
-                                                      let u8_list = x64_encode (Pjcc cond (ucast offset)) in                                                     
-                                                      (x64_bin_update (length u8_list) l_bin0 loc u8_list)))"
-                  using d3 apply(cases "x64_decode (nat ?fix_begin_addr+sz) l_bin0",simp_all)
-                  subgoal for a apply(cases a,simp_all)
-                    subgoal for aa b apply(cases b,simp_all)
-                      subgoal for x131 x132
-                        by (meson option.inject)
-                      done
-                    done
-                  done
-                
-                have "last_fix_sem 2 prog' xst = x64_sem 2 prog' xst" using last_fix_sem_def by simp
-                hence e0_0:"last_fix_sem 2 prog' xst =  (
-                  case x64_decode xpc prog' of
-                  None \<Rightarrow> Stuck |
-                  Some (sz, ins) \<Rightarrow>
-                    x64_sem 1 prog' (exec_instr ins sz xpc xrs xm xss)
-                )"  by (metis Suc_1 a3 x64_sem.simps(3)) 
-
-               (* have "list_in_list (x64_encode(Pcmpq_rr src dst)) xpc l_bin0" using d2 d3_1 
-                proof(rule ccontr)
-                  assume assm:"\<not> (list_in_list (x64_encode(Pcmpq_rr src dst)) xpc l_bin0)"
-                  have "\<not> (x64_decode xpc l_bin0 = Some (length (x64_encode(Pcmpq_rr src dst)), Pcmpq_rr src dst))" using x64_encode_decode_consistency assm 
-                  have e0:"x64_decode xpc prog' = x64_decode xpc l_bin0" 
-                  proof(rule ccontr)*)
-
-                hence e1:"last_fix_sem 2 prog' xst =  (
-                  case x64_decode xpc prog' of
-                  Some (sz, Pcmpq_rr src dst) \<Rightarrow>
-                    x64_sem 1 prog' (exec_instr (Pcmpq_rr src dst) sz xpc xrs xm xss)
-                )" using c0_0 a3 e0_0 apply(cases "x64_decode xpc prog'",simp_all) sorry
-                
-                have "last_fix_sem 2 prog xst = x64_sem 2 prog xst" using last_fix_sem_def by simp
-                hence e0:"last_fix_sem 2 prog xst =  (
-                  case x64_decode xpc prog of
-                  None \<Rightarrow> Stuck |
-                  Some (sz, ins) \<Rightarrow>
-                    x64_sem 1 prog (exec_instr ins sz xpc xrs xm xss)
-                )"
-                  by (metis Suc_1 a3 x64_sem.simps(3)) 
-                have e1:"\<exists> num src dst. x64_decode xpc prog = Some(num, Pcmpq_rr src dst)" sorry
-                hence "\<exists> src dst sz. last_fix_sem 2 prog xst = x64_sem 1 prog (exec_instr (Pcmpq_rr src dst) sz xpc xrs xm xss)"
-                  using e0 e1 by force
-                then obtain src dst sz where e2:"last_fix_sem 2 prog xst = x64_sem 1 prog (exec_instr (Pcmpq_rr src dst) sz xpc xrs xm xss)" by auto
-                hence e3:"sz = 3" using x64_encode_decode_consistency x64_encode_def list_in_list_prop sorry
-
-              then show ?thesis sorry
-            next
-              case False
-              then show ?thesis sorry
-            qed
-      next
-        case False
-        then show ?thesis sorry
-      qed
-    next
-      case False
-      have b1:"(\<not>(\<exists> num d. x64_decode xpc l_bin0 = Some(num, Pcall_i d))) \<and> (\<not>(\<exists> num src dst. x64_decode xpc l_bin0 = Some(num, Pcmpq_rr src dst)))"
-        using False b0 by blast
-      then show ?thesis
-      proof(cases "\<exists> num. x64_decode xpc l_bin0 = Some(num, Pret)")
-        case True
-        then show ?thesis sorry
-      next
-        case False
-        have b0_0:"(\<not>(\<exists> num. x64_decode xpc l_bin0 = Some(num,Pret))) \<and> (\<not>(\<exists> num d. x64_decode xpc l_bin0 = Some(num, Pcall_i d))) \<and> (\<not> (\<exists> num src dst. x64_decode xpc l_bin0 = Some(num, Pcmpq_rr src dst)))"
-          using b1 False by blast
-        
-        have b0_2:"x64_decode xpc l_bin0 \<noteq> None" 
-        proof(rule ccontr)
-          assume assm:"\<not> (x64_decode xpc l_bin0 \<noteq> None)"
-          have "x64_decode xpc l_bin0 = None" using assm by blast          
-          have c0:"snd fxst' =  snd (let num = snd (l_pc!(unat pc)) in (pc+1, x64_sem num l_bin0 (Next xpc xrs xm xss)))" 
-            using b0_0 a1 a3 b0_1 apply(unfold flat_bpf_one_step_def,simp_all)
-            apply(cases "xst",simp_all)
-            apply(split if_splits,simp_all)
-            subgoal for x11 
-            apply(cases "x64_decode xpc l_bin0",simp_all)
-               apply (smt (z3) option.simps(4) outcome.simps(3) snd_conv)
-              subgoal for a
-                using assm by force
-              done
-            done            
-          have "\<exists> num off l. lt!(unat pc) = (num,off,l)" by (metis surj_pair) 
-          then obtain num off l where c0_1:"lt!(unat pc) = (num,off,l)" by auto
-          hence c1:"(snd (l_pc ! unat pc)) = num" using flattern_num a6 a4 c0_1 by fastforce 
-          have "num>0" using a5 well_formed_prog_def a6 c0_1 by force
-          hence "(snd (l_pc ! unat pc)) > 0" using c1 by force
-          hence "snd fxst' = Stuck" using c0 c1 apply(cases "x64_decode xpc l_bin0",simp_all)
-             apply (smt (verit, del_insts) Suc_diff_1 option.simps(4) x64_sem.simps(3)) 
-            subgoal for a using assm by auto
-            done
-          thus "False" using a1 by auto
-        qed
-       
-        hence b0:"snd fxst' = x64_sem (snd (l_pc!(unat pc))) l_bin0 (Next xpc xrs xm xss)"
-          using b0_0 b0_1 b0_2 a1 a3 b1 a6 b0_3 apply(unfold flat_bpf_one_step_def,simp_all)
-            apply(cases "xst",simp_all)
-          subgoal for x11 
-            apply(unfold Let_def)
-            apply(split if_splits,simp_all)
-            apply(split if_splits,simp_all)
-            subgoal for a b apply(cases b,simp_all)
-              done
-            done
-          done
-        have b1:"last_fix_sem (snd (l_pc!(unat pc))) prog xst = x64_sem (snd (l_pc!(unat pc))) prog xst" 
-          using last_fix_sem_def by auto
-        have "\<exists> l. list_in_list l xpc l_bin0 \<longrightarrow> list_in_list l xpc prog" using jit_fix_not_change b0_1 a2 b0_0
-          using list_in_list.simps(1) by metis
-        then obtain l where b2:"list_in_list l xpc l_bin0 \<longrightarrow> list_in_list l xpc prog" by auto
-        thus ?thesis
-        proof(cases "list_in_list l xpc l_bin0")
-          case True
-          have b2:"list_in_list l xpc l_bin0 = list_in_list l xpc prog" using True b2 by simp
-          (*have "x64_decode 0 l = x64_decode xpc l_bin0 \<and> x64_decode 0 l = x64_decode xpc prog" using list_in_list_x64_decode b0_2 sorry
-          hence "x64_decode xpc l_bin0 = x64_decode xpc prog " using list_in_list_x64_decode by argo *)
-          have "x64_bin_is_sequential (length l) l 0" sorry
-          hence "(last_fix_sem (snd (l_pc!(unat pc))) prog xst) = (snd fxst')" 
-          using b0 b1 list_in_list_prop4 a1 by (metis True a3 b2)  
-        hence "\<exists> num fst'. num = (snd (l_pc!(unat pc))) \<and> last_fix_sem num prog xst = fst' \<and> match_state2 fst' (snd fxst')"
-          apply(unfold match_state2_def,simp_all) using a1 a3
-          by(cases "snd fxst'",simp_all)           
-        then show ?thesis by blast
-        next
-          case False
-          then show ?thesis sorry
-        qed
-      qed
-    qed
-  qed
-qed
-
-*)
 
 
 
